thys/Untyped_Lambda_Calculus/LC_Head_Reduction.thy
@@ -3,6 +3,11 @@ imports LC2
 begin
 
 definition red where 
-"red e ee \<equiv> \<exists>x e1 e2. e = App (Lam x e1) e2 \<and> ee = tvsubst (Var(x:=e2)) e1"
+"red (e::trm) ee \<equiv> \<exists>x e1 e2. e = App (Lam x e1) e2 \<and> ee = tvsubst (Var(x:=e2)) e1"
+
+lemma red_determ: 
+"red e e' \<Longrightarrow> red e e'' \<Longrightarrow> e' = e''"
+unfolding red_def  
+by auto (meson Lam_eq_tvsubst)
 
 end
